theories/lib/base.v
@@ -1,0 +1,190 @@
+
+From stdpp Require Import base gmap.
+From Coq Require Import String.
+
+From language Require Export eff_lang.
+
+Global Instance elem_binder_string : (ElemOf binder (list string)) | 10 := 
+  (λ b xs, match b with
+              BAnon => False%type
+            | BNamed x => x ∈ xs
+           end).
+
+Definition cons_maybe {A} (x : binder * A) (xs : list (string * A)) : list (string * A) :=
+  match x with
+    (BAnon, _) => xs
+  | (BNamed x', a) => (x',a) :: xs
+  end.
+Infix "::?" := cons_maybe (at level 60, right associativity) : list_scope.
+
+Lemma binder_delete_union {A} x (vs ws : gmap string A) :
+  binder_delete x (vs ∪ ws) = binder_delete x vs ∪ binder_delete x ws.
+Proof. destruct x; first done; simpl. apply delete_union. Qed.
+
+Global Instance delete_gmap_multiple K A `{ Countable K, EqDecision K, Delete K (gmap K A) } : 
+  Delete (list K) (gmap K A) :=
+  (fix delete_mult xs vs :=
+      match xs with
+        [] => vs
+      | x :: xxs => delete x (delete_mult xxs vs)
+      end).
+
+Lemma delete_list_nil {A} (vs : gmap string A) :
+  delete [] vs = vs.
+Proof. done. Qed.
+
+Lemma delete_list_cons {A} x (xs : list string) (vs : gmap string A) :
+  delete (x :: xs) vs = delete x (delete xs vs).
+Proof. done. Qed.
+
+Lemma delete_list_delete {A} x (vs : gmap string A) :
+  delete [x] vs = delete x vs.
+Proof. done. Qed.
+
+Lemma delete_list_empty {A} (xs : list string) :
+  delete xs ∅ = (∅ : gmap string A).
+Proof.
+  induction xs; first done. 
+  by rewrite delete_list_cons IHxs delete_empty.
+Qed.
+
+Lemma delete_list_commute {A}
+  (x : string) (xs : list string) (vs : gmap string A) :
+  delete x (delete xs vs) = delete xs (delete x vs).
+Proof.
+  induction xs; first done.
+  assert (Hrw : ∀ (vs : gmap string A), delete (a :: xs) vs = delete a (delete xs vs)) by (by intros ?).
+  rewrite !Hrw.
+  by rewrite delete_commute IHxs.
+Qed.
+
+Lemma delete_list_singleton {A} (z : string) (xs : list string) (m : A) :
+  z ∈ xs → delete xs {[z:=m]} = (∅ : gmap string A).
+Proof.
+  intros ?. induction xs; simpl; [inversion H|].
+  set g := {[z := m]}.
+  rewrite delete_list_cons.
+  destruct (decide (z = a)).
+  - subst. by rewrite delete_list_commute delete_singleton delete_list_empty. 
+  - rewrite IHxs; first (apply delete_empty). 
+    destruct (elem_of_cons xs z a) as [H' _].
+    by edestruct H'.
+Qed.
+  
+Lemma delete_list_singleton_ne {A} (z : string) (xs : list string) (m : A) :
+  z ∉ xs → delete xs {[z:=m]} = ({[z:=m]} : gmap string A).
+Proof.
+  intros ?. induction xs; first done.
+  destruct (not_elem_of_cons xs z a) as [[] _]; first done. 
+  rewrite delete_list_cons IHxs; last done. 
+  rewrite delete_insert_ne; last congruence. 
+  by rewrite delete_empty insert_empty.
+Qed.
+
+Lemma lookup_difference_delete {A} z (vs ws : gmap string A) :
+  (vs ∖ delete z ws) !! z = vs !! z.
+Proof.
+  destruct (vs !! z) eqn:H.
+  - rewrite (difference_delete _ _ _ a); last done.
+    by rewrite lookup_insert.
+  - apply lookup_difference_None; auto.
+Qed.
+
+Lemma lookup_difference_delete_ne {A} i j (vs ws : gmap string A) :
+  i ≠ j → (vs ∖ ws) !! j = (vs ∖ delete i ws) !! j.
+Proof.
+  intros H. destruct (ws !! j) eqn:H'.
+  - destruct (lookup_difference_None vs ws j) as [_ ->]; last auto. 
+    destruct (lookup_difference_None vs (delete i ws) j) as [_ ->]; first done.
+    right. rewrite lookup_delete_ne; auto.
+  - destruct (vs !! j) eqn:?.
+    { destruct (lookup_difference_Some vs ws j a) as [_ ->]; auto.
+      destruct (lookup_difference_Some vs (delete i ws) j a) as [_ ->]; first done.
+      split; first done. rewrite lookup_delete_ne; auto. }
+    destruct (lookup_difference_None vs ws j) as [_ ->]; auto.
+    destruct (lookup_difference_None vs (delete i ws) j) as [_ ->]; auto.
+Qed.
+
+Lemma delete_list_delete_cons {A} (z : string) (xs : list string) (vs : gmap string A) :
+  z ∈ xs → delete xs vs = delete (z :: xs) vs.
+Proof.
+  intros H. induction xs; [inversion H|].
+  rewrite !delete_list_cons.
+  destruct (elem_of_cons xs z a) as [[] _]; first done.
+  - subst. by rewrite delete_idemp.
+  - rewrite delete_commute. rewrite delete_list_cons in IHxs.
+    by rewrite -IHxs.
+Qed.
+
+Lemma delete_list_elem_of (Γ : list string) x (vs : gmap string val) :
+  x ∈ Γ → delete Γ vs = delete x (delete Γ vs).
+Proof.
+  intros Helem. induction Γ.
+  { by destruct (not_elem_of_nil x). }
+  destruct (decide (a = x)); first subst. 
+  { by rewrite delete_idemp. }
+  rewrite delete_commute -IHΓ; first done.
+  by destruct (elem_of_cons Γ x a) as [[] _].
+Qed.
+
+Lemma lookup_delete_not_elem {A} (ys : list string) x (vs : gmap string A) : 
+  x ∉ ys → delete ys vs !! x = vs !! x.
+Proof.
+  intros ?.
+  induction ys; first done.
+  rewrite delete_list_cons.
+  edestruct (not_elem_of_cons ys) as [[] _]; first done.
+  rewrite lookup_delete_ne; last done.
+  by apply IHys. 
+Qed.
+
+Lemma lookup_union_delete_disjoint {A} (xs : list string) x (vs ws : gmap string A) :
+  x ∉ xs → (vs ∪ ws ∖ delete xs ws) !! x = vs !! x.
+Proof.
+  intros ?.
+  induction xs.
+  { by rewrite delete_list_nil map_difference_diag map_union_empty. }
+  edestruct (not_elem_of_cons xs) as [[] _]; first done. 
+  rewrite delete_list_cons. 
+  specialize (IHxs H1).
+  destruct (vs !! x) eqn:H'.
+  { by rewrite lookup_union_l. }
+  apply lookup_union_None; split; first done.
+  rewrite -lookup_difference_delete_ne; last done.
+  erewrite lookup_union_None in IHxs. tauto.
+Qed.
+
+Lemma subset_cons_elem {A} (x : A) xs ys : 
+  x :: xs ⊆ ys → x ∈ ys.
+Proof.
+  intros ?.
+  destruct (elem_of_subseteq (x :: xs) ys) as [H' _].
+  apply H'; first done. rewrite elem_of_cons; by left. 
+Qed.
+
+Lemma subset_cons {A} (x : A) xs ys : 
+  x :: xs ⊆ ys → xs ⊆ ys.
+Proof.
+  intros Hseq. 
+  apply (elem_of_subseteq xs ys). intros z Hz.
+  apply (elem_of_subseteq (x :: xs) ys); first done.
+  apply elem_of_cons. by right.
+Qed.
+
+Lemma disjoint_cons_not_elem {A} (x : A) xs ys : 
+  x :: xs ## ys → x ∉ ys.
+Proof.
+  intros ?.
+  destruct (elem_of_disjoint (x :: xs) ys) as [H' _].
+  intros ?. eapply H'; try done. 
+  rewrite elem_of_cons; by left. 
+Qed.
+
+Lemma disjoint_cons {A} (x : A) xs ys : 
+  x :: xs ## ys → xs ## ys.
+Proof.
+  intros Hseq. 
+  apply (elem_of_disjoint xs ys). intros z Hz.
+  apply (elem_of_disjoint (x :: xs) ys); first done.
+  apply elem_of_cons. by right.
+Qed.
