theories/logic/adequacy.v
@@ -10,8 +10,9 @@ From program_logic Require Import weakest_precondition
                                   tactics.
 (* Local imports *)
 From affine_tes.lang Require Import hazel.
+From affine_tes.lang Require Import subst_map.
+From affine_tes.logic Require Import sem_def.
 From affine_tes.logic Require Import sem_types.
-From affine_tes.logic Require Import sem_typed.
 
 (* This file is largely based from the adequacy proof in TES:
    https://gitlab.inria.fr/cambium/tes/-/blob/main/theories/logic/adequacy.v
