theories/logic/sem_env.v
@@ -1,0 +1,218 @@
+
+From iris.proofmode Require Import base tactics classes.
+From iris.program_logic Require Import weakestpre.
+
+From stdpp Require Import base gmap.
+
+(* Hazel Reasoning *)
+From program_logic Require Import weakest_precondition 
+                                  state_reasoning.
+
+(* Local imports *)
+From affine_tes.lib Require Import base.
+From affine_tes.lang Require Import hazel.
+From affine_tes.lang Require Import subst_map.
+From affine_tes.logic Require Import iEff.
+From affine_tes.logic Require Import sem_def.
+From affine_tes.logic Require Import sem_types.
+
+Lemma env_dom_nil {Σ} :
+  env_dom (Σ:= Σ) [] = [].
+Proof. done. Qed.
+
+Lemma env_dom_cons {Σ} x τ (Γ : env Σ) :
+  env_dom ((x, τ) :: Γ) = x :: env_dom Γ.
+Proof. done. Qed.
+
+Lemma env_dom_app {Σ} (Γ₁ Γ₂ : env Σ) :
+  env_dom (Γ₁ ++ Γ₂) = env_dom Γ₁ ++ env_dom Γ₂.
+Proof. by rewrite -map_app. Qed.
+
+Lemma env_sem_typed_empty `{irisGS eff_lang Σ} vs : ⟦ [] ⟧ vs = True%I.
+Proof. done. Qed.
+
+Lemma env_sem_typed_cons `{irisGS eff_lang Σ} x τ Γ' vs : 
+    ⟦ (x, τ) :: Γ' ⟧ vs = ((∃ v, ⌜ vs !! x = Some v ⌝ ∗ τ v) ∗ ⟦ Γ' ⟧ vs)%I.
+Proof. done. Qed.
+
+Lemma env_sem_typed_insert `{irisGS eff_lang Σ} Γ vs (x : string) v :
+  x ∉ (env_dom Γ) →
+  ⟦ Γ ⟧ vs ⊣⊢ ⟦ Γ ⟧ (binder_insert x v vs).
+Proof.
+  intros Helem. 
+  iInduction Γ as [|[y τ] Γ'] "IH";
+    first (iSplit; iIntros; by rewrite env_sem_typed_empty). 
+  rewrite !env_sem_typed_cons; iSplit; iIntros "Henv";
+  iDestruct ("Henv") as "((%w & %Hvs & Hw) & HΓ')".
+  assert (x ≠ y).
+  { rewrite env_dom_cons in Helem.
+    destruct (not_elem_of_cons (env_dom Γ') x y) as [[ ] _]; done. }
+  - iSplitL "Hw".
+    + iExists _. iIntros "{$Hw} !%". 
+      destruct (decide (y = x)) as [->|]. 
+      { destruct Helem. rewrite env_dom_cons. apply elem_of_list_here. }
+      by rewrite lookup_insert_ne.
+    + iApply "IH"; last done. iPureIntro. 
+      destruct (not_elem_of_cons (env_dom Γ') x y) as [[ ] _]; done.
+  - iSplitL "Hw".
+    + iExists w.  iIntros "{$Hw} !%". 
+      destruct (decide (y = x)) as [->|]. 
+      { destruct Helem. rewrite env_dom_cons. apply elem_of_list_here. }
+      by rewrite lookup_insert_ne in Hvs.
+    + iApply "IH"; last done. iPureIntro. 
+      destruct (not_elem_of_cons (env_dom Γ') x y) as [[ ] _]; done.
+Qed.
+
+Ltac solve_sem_typed_insert :=
+  rewrite env_sem_typed_insert; try (simplify_eq; done); progress iFrame "%#∗".
+
+Ltac solve_sem_typed_insert_inv :=
+  rewrite -env_sem_typed_insert; try (simplify_eq; done); progress iFrame "%#∗".
+
+Ltac solve_env := 
+  repeat (
+    done ||
+    iIntros || 
+    iExists _ || 
+    iPureIntro ||
+    iSplit || 
+    (progress iFrame "%#∗") ||
+    (progress simpl) ||
+    apply lookup_insert || 
+    rewrite lookup_insert_ne || 
+    apply lookup_delete ||
+    rewrite env_sem_typed_empty ||
+    rewrite env_sem_typed_cons ||
+    solve_sem_typed_insert ||
+    solve_sem_typed_insert_inv
+  ).
+
+Lemma env_sem_typed_union `{irisGS eff_lang Σ} Γ ws vs :
+  ⟦ Γ ⟧ vs ⊢ ⟦ Γ ⟧ (vs ∪ ws).
+Proof. 
+  iIntros "HΓ". iInduction Γ as [|[x τ] Γ'] "IH"; first done.
+  rewrite !env_sem_typed_cons.
+  iDestruct "HΓ" as "[(%m & %Hrw & Hx) HΓ']".
+  rewrite -/env_sem_typed. 
+  iSplitL "Hx"; [|by iApply "IH"].
+  iExists m; iFrame; iPureIntro.
+  by rewrite lookup_union_l.
+Qed.
+
+Lemma env_sem_typed_delete_union `{irisGS eff_lang Σ} Γ (Δ : env Σ) ws vs :
+  env_dom Γ ⊆ env_dom Δ →
+  ⟦ Γ ⟧ vs ⊣⊢ ⟦ Γ ⟧ (delete (env_dom Δ) ws ∪ vs).
+Proof.
+  intros ?. iSplit.
+  - iInduction Γ as [|[x τ] Γ'] "IH"; first solve_env. 
+    rewrite !env_sem_typed_cons.
+    iIntros "/= [(%w & %Hrw & Hw) HΓ']".
+    assert (Hseq' : env_dom Γ' ⊆ env_dom Δ). 
+    { eapply subset_cons. by erewrite <- env_dom_cons. }
+    assert (x ∈ (env_dom Δ)).
+    { eapply subset_cons_elem. by erewrite <- env_dom_cons. }
+    iSplitL "Hw";[| iApply ("IH" with "[] HΓ'"); by iPureIntro].
+    iExists w. iFrame. iPureIntro. 
+    rewrite (delete_list_elem_of _ x); last done.
+    rewrite lookup_union_r; first done. apply lookup_delete.
+  - iInduction Γ as [|[x τ] Γ'] "IH"; first solve_env.
+    rewrite !env_sem_typed_cons.
+    iIntros "[(%v & %Hrw & Hτ) HΓ']".
+    iSplitL "Hτ".
+    + iExists v. iIntros "{$Hτ} !%".
+      rewrite -(lookup_union_r (delete (env_dom Δ) ws)); first done.
+      rewrite (delete_list_elem_of _ x); first (apply lookup_delete).
+      eapply subset_cons_elem. by erewrite <- env_dom_cons.
+    + iApply "IH"; last done.
+      iPureIntro. eapply subset_cons. by erewrite <- env_dom_cons.
+Qed.
+
+Lemma env_sem_typed_difference_delete `{irisGS eff_lang Σ} Γ (Δ : env Σ) vs ws :
+  env_dom Γ ⊆ env_dom Δ → ⟦ Γ ⟧ vs ⊣⊢ ⟦ Γ ⟧ (vs ∖ delete (env_dom Δ) ws).
+Proof.
+  intros ?.
+  iInduction Γ as [|[x τ] Γ'] "IH"; first (iSplit; solve_env).
+  rewrite !env_sem_typed_cons; iSplit;
+  iIntros "/= [(%v & %Hrw & Hτ) HΓ']".
+  assert (Hseq' : env_dom Γ' ⊆ env_dom Δ).
+  { eapply subset_cons. by erewrite <- env_dom_cons. }
+  assert (x ∈ (env_dom Δ)).
+  { eapply subset_cons_elem. by erewrite <- env_dom_cons. }
+  - iSplitL "Hτ".
+    + iExists _. iFrame. iPureIntro. 
+      rewrite (delete_list_elem_of _ x); last done. 
+      by rewrite lookup_difference_delete. 
+    + iApply ("IH" with "[] HΓ'"); eauto. 
+  - iSplitL "Hτ".
+    + iExists _. iFrame. iPureIntro. 
+      rewrite (delete_list_elem_of _ x) in Hrw; 
+        [|eapply subset_cons_elem; by erewrite <- env_dom_cons].
+      by rewrite lookup_difference_delete in Hrw.
+    + iApply ("IH" with "[] HΓ'"); eauto. 
+      iPureIntro. eapply subset_cons. by erewrite <- env_dom_cons.
+Qed.
+
+Lemma env_sem_typed_delete_disjoint `{irisGS eff_lang Σ} Γ (Δ : env Σ) vs  :
+  env_dom Γ ## env_dom Δ → ⟦ Γ ⟧ vs ⊣⊢ ⟦ Γ ⟧ (delete (env_dom Δ) vs).
+Proof. 
+  iIntros (?).
+  iInduction Γ as [|[x τ] Γ'] "IH"; first (iSplit; solve_env). 
+  rewrite !env_sem_typed_cons; iSplit;
+  iIntros "/= [(%v & %Hrw & Hτ) HΓ']";
+  assert (Hseq' : env_dom Γ' ## env_dom Δ)
+    by (eapply disjoint_cons; by erewrite <- env_dom_cons);
+  assert (x ∉ (env_dom Δ)) by 
+    (eapply disjoint_cons_not_elem; by erewrite <- env_dom_cons).
+  - iSplitL "Hτ".
+    + iExists v. iIntros "{$Hτ} !%".
+      by rewrite lookup_delete_not_elem.
+    + by iApply "IH".
+  - iSplitL "Hτ".
+    + iExists v. iIntros "{$Hτ} !%".
+      by rewrite lookup_delete_not_elem in Hrw.
+    + by iApply "IH".
+Qed. 
+
+Lemma env_sem_typed_union_difference_delete `{irisGS eff_lang Σ} Γ (Δ : env Σ) vs ws :
+  env_dom Γ ## env_dom Δ → ⟦ Γ ⟧ (vs ∪ ws ∖ (delete (env_dom Δ) ws)) ⊢ ⟦ Γ ⟧ vs.
+Proof. 
+  intros ?.
+  iInduction Γ as [|[x τ] Γ'] "IH"; first solve_env.
+  rewrite !env_sem_typed_cons.
+  iIntros "/= [(%v & %Hrw & Hτ) HΓ']".
+  assert (Hseq' : env_dom Γ' ## env_dom Δ)
+    by (eapply disjoint_cons; by erewrite <- env_dom_cons).
+  assert (x ∉ (env_dom Δ)) by 
+    (eapply disjoint_cons_not_elem; by erewrite <- env_dom_cons).
+  iSplitL "Hτ".
+  + iExists v. iIntros "{$Hτ} !%".
+    by rewrite lookup_union_delete_disjoint in Hrw.
+  + by iApply "IH".
+Qed.
+
+Lemma env_sem_typed_app `{irisGS eff_lang Σ} Γ₁ Γ₂ vs :
+  ⟦ Γ₁ ++ Γ₂ ⟧ vs ⊣⊢ ⟦ Γ₁ ⟧ vs ∗ ⟦ Γ₂ ⟧ vs.
+Proof. 
+  iInduction Γ₁ as [|[y τ] Γ₁'] "IH". 
+  { iSplit; [iIntros; by iFrame|iIntros "[_ H] {$H}"]. }
+  iSplit; rewrite !env_sem_typed_cons; iIntros "HΓ₁₂". 
+  - iDestruct "HΓ₁₂" as "($ & HΓ₁'₂)". by iApply "IH".
+  - iDestruct ("HΓ₁₂") as "[[Hτ HΓ₁'] HΓ₂]".
+    rewrite -/app. iFrame. iApply ("IH" with "[HΓ₁' HΓ₂]").
+    iFrame.
+Qed.
+
+Lemma env_sem_typed_mk_moved `{irisGS eff_lang Σ} vs Γ :
+  ⟦ Γ ⟧ vs -∗
+  □ ⟦ map (prod_map id (const Moved)) Γ ⟧ vs ∗ ⟦ Γ ⟧ vs.
+Proof.
+  iIntros "HΓ". iInduction Γ as [|x Γ'] "IH"; first done. simpl.
+  destruct x. simpl. rewrite !env_sem_typed_cons.
+  iDestruct "HΓ" as "[(%w & -> & Hw) HΓ']". 
+  iSpecialize ("IH" with "HΓ'"). 
+  rewrite bi.intuitionistically_sep.
+  rewrite -bi.sep_assoc. iSplitR.
+  { by iExists w. }
+  iDestruct "IH" as "[HΓ'T HΓ']". iFrame.
+  { iExists w. by iFrame. }
+Qed.
