theories/logic/sem_operators.v
@@ -1,5 +1,6 @@
 
 From affine_tes.lang Require Import hazel.
+From affine_tes.logic Require Import sem_def.
 From affine_tes.logic Require Import sem_types.
 
 Open Scope sem_ty_scope.
